1. Formulieren Sie das System in der Form

\begin{equation*}
	u' = F(t,u)
\end{equation*}

Die Randbedingungen

\begin{equation}
	D\cdot \frac{\partial u}{\partial z}(0)=S_Lu(0),\quad D\frac{\partial u}{\partial z}(d)=-S_Ru(d)
\end{equation}

und:

\begin{align*}
	&k=k_1+k_2\cdot N_D\\
	&s_i=s(z_i)\\
	&h=\frac{d}{N}\\
	&u(i)\approx u_i
\end{align*}

Analog wie im zweiten Abschnitt

\begin{equation}
	\frac{\partial^2 u}{\partial z^2}(t,z_i) = \frac{u_{i+1}(t) - 2\cdot u_i(t) + u_{i-1}(t)}{h^2}
\end{equation}

\begin{equation}
	\frac{\partial u}{\partial t}(t,z_i) =\frac{\partial^2 u}{\partial z^2}(t,z_i)- \frac{u_{i+1}(t) - (k_1 + K_2N_D)\cdot u(t,z_i)}{h^2} - k_2\cdot u^2(t,z_i) + s(t,z_i)
\end{equation}
	
\begin{equation}
		\frac{\partial u}{\partial t}(t,z_i) = D\cdot \frac{u_{i+1}(t) - 2\cdot u_i(t) + u_{i-1}(t)}{h^2} - ku_i(t) - K_2u^2_i(t) + s_i(t)
\end{equation}
	
\begin{equation}
		\frac{\partial u}{\partial t}(t,z_i) = 	\frac{D}{h^2}u_{i+1}(t) - 2\cdot \frac{D}{h^2}u_i(t) + \frac{D}{h^2}u_{i-1}(t) - ku_i(t) - K_2u^2_i(t) + s_i(t)
\end{equation}
	
\begin{equation}
		\frac{\partial u}{\partial t}(t,z_i) = 	\frac{D}{h^2}u_{i+1}(t) - (2\cdot \frac{D}{h^2} + k)u_i(t) + \frac{D}{h^2}u_{i-1}(t) - K_2u^2_i(t) + s_i(t)
\end{equation}
	
	
Nun werden die Gleichungen f√ºr $z_0$ und $z_N$ hergeleitet:
	
\begin{equation}
		\frac{\partial u}{\partial t}(z_i) = \frac{u_{i+1}(t) - u_{i-1}(t)}{2\cdot h}\\
		u'(0) \sim \frac{u_1-u_{-1}}{2\cdot h}, \quad u'(d) \sim \frac{u_N+1-u_{N-1}}{2\cdot h}
\end{equation}